lec5

wrapper/main.c
@@ -1,9 +1,26 @@
 #include <stdio.h>
 
+const int BOOL_TAG   = 0x00000001;
+const int BOOL_TRUE  = 0x80000001; // These must be the same values
+const int BOOL_FALSE = 0x00000001; // as chosen in compile.ml
+
+int print(int val) {
+  if ((val & BOOL_TAG) == 0) { // val is even ==> number
+    printf("%d", val >> 1); // shift bits right to remove tag
+  } else if (val == BOOL_TRUE) {
+    printf("true");
+  } else if (val == BOOL_FALSE) {
+    printf("false");
+  } else {
+    printf("Unknown value: %#010x", val); // print unknown val in hex
+  }
+  return val;
+}
+
 extern int our_code_starts_here() asm("our_code_starts_here");
 
 int main(int argc, char** argv) {
   int result = our_code_starts_here();
-  printf("%d", result);
+  print(result);
   return 0;
 }
