Cs4410sp19/Basic.lean
@@ -17,10 +17,20 @@ inductive Instruction where
   | add : Arg → Arg → Instruction
   | sub : Arg → Arg → Instruction
   | mul : Arg → Instruction
+  | shl : Arg → Arg → Instruction
+  | shr : Arg → Arg → Instruction
+  | sar : Arg → Arg → Instruction
+  | and : Arg → Arg → Instruction
+  | or : Arg → Arg → Instruction
+  | xor : Arg → Arg → Instruction
   | label : String → Instruction
   | cmp : Arg → Arg → Instruction
   | jmp : String → Instruction
   | je : String → Instruction
+  | jl : String → Instruction
+  | jle : String → Instruction
+  | jg : String → Instruction
+  | jge : String → Instruction
 deriving Inhabited
 
 instance : ToString Reg where
@@ -40,33 +50,52 @@ instance : ToString Instruction where
   | .add dst src => s!"add {dst}, {src}"
   | .sub dst src => s!"sub {dst}, {src}"
   | .mul src => s!"mul {src}"
+  | .shl dst bits => s!"shl {dst}, {bits}"
+  | .shr dst bits => s!"shr {dst}, {bits}"
+  | .sar dst bits => s!"sar {dst}, {bits}"
+  | .and dst src => s!"and {dst}, {src}"
+  | .or dst src => s!"or {dst}, {src}"
+  | .xor dst src => s!"xor {dst}, {src}"
   | .label name => s!"{name}:"
   | .cmp x y => s!"cmp {x}, {y}"
   | .jmp name => s!"jmp {name}"
   | .je name => s!"je {name}"
+  | .jl name => s!"jl {name}"
+  | .jle name => s!"jle {name}"
+  | .jg name => s!"jg {name}"
+  | .jge name => s!"jge {name}"
 
 def asm_to_string : Array Instruction → String := fun xs =>
   String.intercalate "\n" (xs.map toString).toList
 
+inductive Prim1 where
+  | neg | not
+deriving Inhabited, Repr
+
 inductive Prim2 where
   | plus | minus | times
+  | land | lor | lt | le | gt | ge | eq | ne
 deriving Inhabited, Repr
 
 inductive Expr where
   | num : Int → Expr
   | id : String → Expr
   | let_in : String → Expr → Expr → Expr
+  | prim1 : Prim1 → Expr → Expr
   | prim2 : Prim2 → Expr → Expr → Expr
   | ite : Expr → Expr → Expr → Expr
+  | bool : Bool → Expr
 deriving Inhabited, Repr
 
 def Expr.is_imm (e : Expr) : Bool :=
   match e with
   | .num _ | .id _ => true
+  | .bool .true | .bool .false => true
   | _ => false
 
 def Expr.is_anf (e : Expr) : Bool :=
   match e with
+  | .prim1 _ x => x.is_imm
   | .prim2 _ x y => x.is_imm && y.is_imm
   | .let_in _ v k => v.is_anf && k.is_anf
   | .ite cond bp bn => cond.is_imm && bp.is_anf && bn.is_anf
@@ -75,9 +104,13 @@ def Expr.is_anf (e : Expr) : Bool :=
 inductive Expr.IsImm : Expr → Prop where
   | num x : IsImm (.num x)
   | id name : IsImm (.id name)
+  | bool x : IsImm (.bool x)
+
+attribute [simp] Expr.IsImm.num Expr.IsImm.id Expr.IsImm.bool
 
 inductive Expr.IsANF : Expr → Prop where
   | of_imm {e} : Expr.IsImm e → e.IsANF
+  | prim1 {op : Prim1} {x : Expr} : x.IsImm → (Expr.prim1 op x).IsANF
   | prim2 {op : Prim2} {x y : Expr} : x.IsImm → y.IsImm → (Expr.prim2 op x y).IsANF
   | let_in {name} {v k : Expr} : v.IsANF → k.IsANF → (Expr.let_in name v k).IsANF
   | ite {cond bp bn : Expr} : cond.IsImm → bp.IsANF → bn.IsANF → (Expr.ite cond bp bn).IsANF
