Cs4410sp19/Parser.lean
@@ -12,6 +12,15 @@ private def atom : String → Parser Unit := fun x => pstring x *> ws
 /-- useful for trailing parsers (e.g. binary operators) -/
 private partial def fix (cont : α → Parser α) : α → Parser α := fun c => (cont c >>= fix cont) <|> pure c
 
+def parse_infixl (ops : List (String × Prim2)) (next : Parser Expr) : Parser Expr := do
+  let head ← next
+  ws
+  assert! ops.length != 0
+  let op :: ops := ops | unreachable!
+  let gen := fun (op, op') => fun c => pstring op *> ws *> (Expr.prim2 op' c <$> next) <* ws
+  let ts := ops.foldl (α := Expr → Parser Expr) (β := String × Prim2) (init := gen op) fun acc x => (fun t => acc t <|> (gen x) t)
+  fix ts head
+
 variable (pe : Parser Expr)
 mutual
 
@@ -55,21 +64,31 @@ partial def parse_expr_inner : Parser Expr := do
   attempt (Expr.num <$> parse_num_val)
   <|> attempt parse_let_in <|> attempt parse_ite
   <|> attempt (pchar '(' *> ws *> pe <* ws <* pchar ')' <* ws)
+  <|> attempt (atom "true" *> pure (.bool .true))
+  <|> attempt (atom "false" *> pure (.bool .false))
   <|> attempt (Expr.id <$> parse_ident)
 
-partial def parse_mul : Parser Expr := do
-  let head ← parse_expr_inner
-  ws
-  fix (fun c => pchar '*' *> ws *> (.prim2 .times c <$> parse_expr_inner) <* ws) head
+partial def parse_neg : Parser Expr := do
+  attempt (atom "-" *> Expr.prim1 .neg <$> parse_expr_inner) <|> parse_expr_inner
 
-partial def parse_add_sub : Parser Expr := do
-  let head ← parse_mul
-  ws
-  fix (fun c =>
-    (pchar '+' *> ws *> (.prim2 .plus c <$> parse_mul) <* ws)
-    <|> (pchar '-' *> ws *> (.prim2 .minus c <$> parse_mul) <* ws)) head
+partial def parse_not : Parser Expr := do
+  attempt (atom "!" *> Expr.prim1 .not <$> parse_neg) <|> parse_neg
 
-partial def parse_expr_outer : Parser Expr := parse_add_sub
+partial def parse_mul : Parser Expr := parse_infixl [("*", .times)] parse_not
+
+partial def parse_add_sub : Parser Expr := parse_infixl [("+", .plus), ("-", .minus)] parse_mul
+
+partial def parse_hcmp : Parser Expr := parse_infixl (next := parse_add_sub)
+  [("<=", .le), (">=", .ge), ("<", .lt), (">", .gt)]
+
+partial def parse_mcmp : Parser Expr := parse_infixl (next := parse_hcmp)
+  [("==", .eq), ("!=", .ne)]
+
+partial def parse_land : Parser Expr := parse_infixl (next := parse_mcmp) [("&&", .land)]
+
+partial def parse_lor : Parser Expr := parse_infixl (next := parse_land) [("||", .lor)]
+
+partial def parse_expr_outer : Parser Expr := parse_lor
 
 end
 
